BourbakiLean2/Order/WellOrderIso.lean
@@ -4,3 +4,160 @@ variable {α β : Type*} [WellOrder α] [WellOrder β]
 
 theorem WellOrder.either_embeds :
     (∃ x : InitialSegment β, ∃ f : α → x.val, IsOrderIso f) ∨ (∃ x : InitialSegment α, ∃ f : x.val → β, IsOrderIso f) := by
+  let s : Set (PartialMap α $ fun _ => β) := { f | f.carrier.IsDownwardsClosed ∧ StrictMonotone f.function ∧ (f.function '' Set.univ).IsDownwardsClosed}
+  have ind : InductiveOrder s := by
+    constructor
+    intro t h
+    let t' := Subtype.val '' t
+    have ht' : ∀ x, x ∈ t' → ∀ y, y ∈ t' → Comparable x y := by
+        intro x hx y hy
+        unfold t' at hx hy
+        rw[Set.mem_image_iff] at hx hy
+        obtain ⟨⟨x,hx⟩,rfl,hx'⟩ := hx
+        obtain ⟨⟨y,hy⟩,rfl,hy'⟩ := hy
+        exact h ⟨x,hx⟩ hx' ⟨y,hy⟩ hy'
+    have hcurried := (fun (i : t) (j : t) => h i.val i.property j.val j.property)
+    obtain ⟨ub,least⟩ := PartialMap.iUnion_lub (f := fun (x : t) => x.val.val) hcurried
+    have fins : (PartialMap.iUnion fun x : t ↦ x.val.val) ∈ s := by
+        constructor
+        · simp only [PartialMap.iUnion]
+          have : ∀ x : t, x.val.val.carrier.IsDownwardsClosed := by
+            intro ⟨⟨x,mems⟩,mem⟩
+            exact mems.1
+          apply @Set.IsDownwardsClosed.iUnion
+        · constructor
+          · intro ⟨x,⟨tx,hx⟩⟩ ⟨y,⟨ty,hy⟩⟩ h'
+            rcases (h tx.val tx.property ty.val ty.property) with (h|h)
+            · have := (ub ty.val.val Set.val_mem_image_univ).2
+              rw[this x $ h.1 hx, this y $ hy]
+              apply ty.val.property.2.1
+              exact h'
+            · have := (ub tx.val.val Set.val_mem_image_univ).2
+              rw[this y $ h.1 hy, this x $ hx]
+              apply tx.val.property.2.1
+              exact h'
+          · constructor
+            intro b1 b2 le mem
+            obtain ⟨fnc,a,rfl⟩ : ∃ a : t, ∃ x, a.val.val.function x = b2 := by
+                simp only [PartialMap.iUnion, Set.mem_image_iff, Set.mem_univ, and_true,
+                  Subtype.exists, Set.mem_iUnion_iff, exists_prop, exists_and_right] at mem
+                obtain ⟨a,h,rfl⟩ := mem
+                exact ⟨_,_,rfl⟩
+            have : b1 ∈ (fnc.val.val.function '' Set.univ) := by
+                apply fnc.val.property.2.2.mem_of_le_mem le Set.val_mem_image_univ
+            rw[Set.mem_image_iff] at this
+            rw[Set.mem_image_iff]
+            obtain ⟨x,rfl,_⟩ := this
+            exists ⟨x.val,⟨_,x.property⟩⟩
+            simp only [(ub fnc.val.val Set.val_mem_image_univ).2 x.val x.property, Set.mem_univ,
+              and_self]
+    exists ⟨_,fins⟩
+    intro ⟨d,g⟩ hg
+    apply ub
+    simp only [Set.mem_image_iff, Set.mem_univ, and_true, Subtype.exists, exists_prop,
+      exists_and_right, exists_eq_right', hg, g, exists_const]
+  obtain ⟨⟨x,xs⟩,xmax⟩ := ind.has_maximal
+  simp only [StrictMonotone, Subtype.lt_iff_val, Subtype.forall, Set.mem_setOf_iff, s] at xs
+  suffices alt : x.carrier = Set.univ ∨ x.function '' Set.univ = Set.univ by
+    rcases alt with (eq|eq)
+    · left
+      exists ⟨x.function '' Set.univ, xs.2.2⟩
+      exists Function.corestrict (fun a => (x.function ⟨a, eq ▸ Set.mem_univ⟩)) (by
+        intro b h
+        rw[Set.mem_image_iff] at h
+        obtain ⟨a,rfl,_⟩ := h
+        simp only [Set.val_mem_image_univ])
+      apply TotalOrder.strictMono_iso_image
+      · intro a b h
+        exact xs.2.1 a (by simp only [eq, Set.mem_univ]) b (by simp only [eq, Set.mem_univ]) h
+      · simp only [Function.surj_iff, Subtype.eq_iff, Function.coe_corestrict, Subtype.forall,
+        Set.mem_image_iff, Set.mem_univ, and_true, Subtype.exists, forall_exists_index]
+        rintro b a ha rfl
+        exists a
+    · right
+      exists ⟨x.carrier, xs.1⟩
+      exists x.function
+      apply TotalOrder.strictMono_iso_image
+      · intro a b h
+        exact xs.2.1 a.val a.property b.val b.property h
+      · rw[Function.Surjective, eq]
+  by_contra h
+  simp only [not_or] at h
+  obtain ⟨enda, eqa⟩ := isIio_of_downwardsClosed xs.1 h.1
+  obtain ⟨endb,eqb⟩ := isIio_of_downwardsClosed xs.2.2 h.2
+  classical
+  let yfunc : Set.Iic enda → β := fun a =>
+    if h : a.val ∈ x.carrier then x.function ⟨a.val, h⟩ else endb
+  let yf : PartialMap α (fun x => β) := ⟨Set.Iic enda, yfunc⟩
+  have yf1 : yf.carrier.IsDownwardsClosed := by
+    simp only
+    infer_instance
+  have yf2 : StrictMonotone yf.function := by
+    rintro ⟨a,ha⟩ ⟨b,hb⟩ h
+    unfold yf at *
+    simp only [yfunc]
+    split <;> rename_i hif1
+    · split <;> rename_i hif2
+      · apply xs.2.1 a (by assumption) b (by assumption) h
+      · rw[eqa] at hif2
+        simp only [Set.mem_Iio_iff, not_gt_iff_le] at hif2
+        have := le_antisymm hb hif2
+        rcases this
+        have : x.function ⟨a,hif1⟩ ∈ Set.Iio endb := by rw[← eqb]; simp only [Set.val_mem_image_univ]
+        exact this
+    · split <;> rename_i hif2
+      · simp only [eqa,Set.mem_Iio_iff, not_gt_iff_le] at hif1
+        have := le_antisymm ha hif1
+        rcases this
+        exact (not_lt_self $ lt_of_le_lt hb h).elim
+      · simp only [eqa,Set.mem_Iio_iff, not_gt_iff_le] at hif1
+        simp only [eqa,Set.mem_Iio_iff, not_gt_iff_le] at hif2
+        rcases (le_antisymm ha hif1)
+        rcases (le_antisymm hb hif2)
+        exact (not_lt_self h).elim
+  have yf3' : (yf.function '' Set.univ) = Set.Iic endb := by
+    ext b
+    simp only [Set.mem_image_iff, Set.mem_univ, and_true, Subtype.exists, Set.mem_Iic_iff, yfunc]
+    constructor
+    · rintro ⟨a,h,h'⟩
+      split at h' <;> rename_i hif2
+      · rw[h']
+        apply le_of_lt
+        change x.function ⟨a,hif2⟩ ∈ Set.Iio endb
+        rw[← eqb]
+        simp only [Set.val_mem_image_univ]
+      · rw[h']
+    · intro h
+      rw[le_iff_lt_or_eq] at h
+      rcases h with (lt|eq)
+      · have : b ∈ x.function '' Set.univ := by rw[eqb]; exact lt
+        rw[Set.mem_image_iff] at this
+        obtain ⟨a,rfl,_⟩ := this
+        exists a
+        have : a.val < enda := by
+          change a.val ∈ Set.Iio enda
+          rw[← eqa]
+          exact a.property
+        exists le_of_lt this
+        simp only [a.property, ↓reduceDIte]
+      · rw[eq]
+        exists enda
+        exists le_rfl
+        have : enda ∉ x.carrier := by rw[eqa]; exact Set.not_mem_Ioi_self
+        simp[this]
+  have yf3 : (yf.function '' Set.univ).IsDownwardsClosed := by
+    rw[yf3']
+    infer_instance
+  have : yf ∈ s := ⟨yf1,⟨yf2,yf3⟩⟩
+  have := xmax ⟨yf,this⟩ (by
+      constructor
+      swap
+      · simp only [eqa, Set.Iio_subset_Iic]
+      · intro a h
+        simp only [h, ↓reduceDIte, yf, yfunc])
+  have : Set.Iio enda = Set.Iic enda := by
+    have : yf = x := Subtype.eq_iff.mp this
+    rw[← eqa, ← this]
+  apply Set.not_mem_Iio_self (a := enda)
+  rw[this]
+  exact Set.mem_Iic_self
